regex/Regex/NFA/Compile/Lemmas.lean
@@ -12,7 +12,7 @@ theorem pushRegex_size_lt {nfa : NFA} {next e} :
   nfa.size < (nfa.pushRegex next e).size := by
   fun_induction pushRegex
   -- star
-  case case9 nfa next greedy e patchAt placeholder compiled split quest ih =>
+  case case9 nfa next greedy e patchAt placeholder compiled split quest patched ih =>
     calc nfa.size
       _ < placeholder.size := by grind
       _ < compiled.size := ih
@@ -24,7 +24,8 @@ theorem pushRegex_size_lt {nfa : NFA} {next e} :
 theorem pushRegex_wf {nfa : NFA} {next e} (wf : nfa.WellFormed) (next_lt : next < nfa.size) :
   (nfa.pushRegex next e).WellFormed := by
   fun_induction pushRegex
-  case case9 nfa next greedy e patchAt placeholder compiled split quest ih =>
+  -- star
+  case case9 nfa next greedy e patchAt placeholder compiled split quest patched ih =>
     have lt₁ : compiled.start < quest.size := by grind
     have lt₂ : next < quest.size := by grind
     have wfCompiled : compiled.WellFormed := ih (pushNode_wf wf (by grind)) (by grind)
@@ -39,6 +40,20 @@ theorem pushRegex_wf {nfa : NFA} {next e} (wf : nfa.WellFormed) (next_lt : next 
 
 theorem compile_wf {e} : (compile e).WellFormed :=
   pushRegex_wf done_WellFormed done_WellFormed.size_lt
+
+@[grind =]
+theorem pushRegex_get_lt {nfa next e} (i : Nat) (h : i < nfa.size) :
+  (pushRegex nfa next e)[i]'(Nat.lt_trans h pushRegex_size_lt) = nfa[i] := by
+  fun_induction pushRegex nfa next e
+  -- star
+  case case9 nfa next greedy e patchAt placeholder compiled split quest patched ih =>
+    have eq : pushRegex nfa next (.star greedy e) = patched := rfl
+    simp only [eq]
+    conv =>
+      lhs
+      rw [get_eq_nodes_get, Array.getElem_setIfInBounds_ne (by grind) (by grind)]
+      rw [←get_eq_nodes_get, pushNode_get_lt i (by grind), ih (by grind), pushNode_get_lt i (by grind)]
+  all_goals grind
 
 end Regex.NFA
 
